Update tainting examples

Network_Security_Policy_Verification/Examples/Tainting/CryptoDB.thy
@@ -12,34 +12,34 @@ case !Graphviz.open_viewer of
   | DoNothing => ()
 *}
 
-definition policy :: "vString list_graph" where
+definition policy :: "string list_graph" where
   "policy \<equiv> \<lparr> nodesL = [
-                        V ''A'', V ''A_encrypter'', V ''A_channel'',
-                        V ''B'', V ''B_encrypter'', V ''B_channel'',
-                        V ''C'', V ''C_encrypter'', V ''C_channel_in'', V ''C_channel_out'', V ''C_decrypter'',
-                        V ''Adversary'',
-                        V ''CryptoDB''],
+                        ''A'', ''A_encrypter'', ''A_channel'',
+                        ''B'', ''B_encrypter'', ''B_channel'',
+                        ''C'', ''C_encrypter'', ''C_channel_in'', ''C_channel_out'', ''C_decrypter'',
+                        ''Adversary'',
+                        ''CryptoDB''],
               edgesL = [
-              (V ''A'', V ''A_encrypter''), (V ''A_encrypter'', V ''A_channel''), (V ''A_channel'', V ''CryptoDB''),
-              (V ''B'', V ''B_encrypter''), (V ''B_encrypter'', V ''B_channel''), (V ''B_channel'', V ''CryptoDB''),
-              (V ''C'', V ''C_encrypter''), (V ''C_encrypter'', V ''C_channel_out''), (V ''C_channel_out'', V ''CryptoDB''),
-              (V ''CryptoDB'', V ''C_channel_in''), (V ''C_channel_in'', V ''C_decrypter''), (V ''C_decrypter'', V ''C'')
+              (''A'', ''A_encrypter''), (''A_encrypter'', ''A_channel''), (''A_channel'', ''CryptoDB''),
+              (''B'', ''B_encrypter''), (''B_encrypter'', ''B_channel''), (''B_channel'', ''CryptoDB''),
+              (''C'', ''C_encrypter''), (''C_encrypter'', ''C_channel_out''), (''C_channel_out'', ''CryptoDB''),
+              (''CryptoDB'', ''C_channel_in''), (''C_channel_in'', ''C_decrypter''), (''C_decrypter'', ''C'')
               ] \<rparr>"
 
 context begin
   private definition "tainiting_host_attributes \<equiv> [
-                           V ''A'' \<mapsto> TaintsUntaints {''A''} {},
-                           V ''A_encrypter'' \<mapsto> TaintsUntaints {} {''A''},
-                           V ''A_channel'' \<mapsto> TaintsUntaints {} {},
-                           V ''B'' \<mapsto> TaintsUntaints {''B''} {},
-                           V ''B_encrypter'' \<mapsto> TaintsUntaints {} {''B''},
-                           V ''B_channel'' \<mapsto> TaintsUntaints {} {},
-                           V ''C'' \<mapsto> TaintsUntaints {''C''} {},
-                           V ''C_encrypter'' \<mapsto> TaintsUntaints {} {''C''},
-                           V ''C_decrypter'' \<mapsto> TaintsUntaints {''C''} {},
-                           V ''C_channel_out'' \<mapsto> TaintsUntaints {} {},
-                           V ''C_channel_in'' \<mapsto> TaintsUntaints {} {},
-                           V ''Adversary'' \<mapsto> TaintsUntaints {} {}
+                           ''A'' \<mapsto> TaintsUntaints {''A''} {},
+                           ''A_encrypter'' \<mapsto> TaintsUntaints {} {''A''},
+                           ''A_channel'' \<mapsto> TaintsUntaints {} {},
+                           ''B'' \<mapsto> TaintsUntaints {''B''} {},
+                           ''B_encrypter'' \<mapsto> TaintsUntaints {} {''B''},
+                           ''B_channel'' \<mapsto> TaintsUntaints {} {},
+                           ''C'' \<mapsto> TaintsUntaints {''C''} {},
+                           ''C_encrypter'' \<mapsto> TaintsUntaints {} {''C''},
+                           ''C_decrypter'' \<mapsto> TaintsUntaints {''C''} {},
+                           ''C_channel_out'' \<mapsto> TaintsUntaints {} {},
+                           ''C_channel_in'' \<mapsto> TaintsUntaints {} {},
+                           ''Adversary'' \<mapsto> TaintsUntaints {} {}
                            ]"
   private lemma "dom (tainiting_host_attributes) \<subseteq> set (nodesL policy)" by(simp add: tainiting_host_attributes_def policy_def)
   definition "Tainting_m \<equiv> new_configured_list_SecurityInvariant SINVAR_LIB_TaintingTrusted \<lparr>
@@ -48,15 +48,15 @@ end
 lemma "wf_list_graph policy" by eval
 
 ML_val{*
-visualize_graph @{context} @{term "[]::vString SecurityInvariant list"} @{term "policy"};
+visualize_graph @{context} @{term "[]::string SecurityInvariant list"} @{term "policy"};
 *}
 
 
 context begin
   private definition "A_host_attributes \<equiv>
-                [V ''A'' \<mapsto> Member,
-                 V ''A_encrypter'' \<mapsto> Member,
-                 V ''A_channel'' \<mapsto> Member
+                [''A'' \<mapsto> Member,
+                 ''A_encrypter'' \<mapsto> Member,
+                 ''A_channel'' \<mapsto> Member
                  ]"
   private lemma "dom A_host_attributes \<subseteq> set (nodesL policy)"
     by(simp add: A_host_attributes_def policy_def)
@@ -67,9 +67,9 @@ end
 
 context begin
   private definition "B_host_attributes \<equiv>
-                [V ''B'' \<mapsto> Member,
-                 V ''B_encrypter'' \<mapsto> Member,
-                 V ''B_channel'' \<mapsto> Member
+                [''B'' \<mapsto> Member,
+                 ''B_encrypter'' \<mapsto> Member,
+                 ''B_channel'' \<mapsto> Member
                  ]"
   private lemma "dom B_host_attributes \<subseteq> set (nodesL policy)"
     by(simp add: B_host_attributes_def policy_def)
@@ -82,16 +82,16 @@ end
 
 context begin
   private definition "C_host_attributes \<equiv>
-                [V ''C_channel_in'' \<mapsto> InboundGateway,
-                 V ''C_decrypter'' \<mapsto> Member,
-                 V ''C'' \<mapsto> Member,
-                 V ''C_encrypter'' \<mapsto> Member,
-                 V ''C_channel_out'' \<mapsto> Member
+                [''C_channel_in'' \<mapsto> InboundGateway,
+                 ''C_decrypter'' \<mapsto> Member,
+                 ''C'' \<mapsto> Member,
+                 ''C_encrypter'' \<mapsto> Member,
+                 ''C_channel_out'' \<mapsto> Member
                  ]"
   private lemma "dom C_host_attributes \<subseteq> set (nodesL policy)"
     by(simp add: C_host_attributes_def policy_def)
   definition "SystemC_m \<equiv> new_configured_list_SecurityInvariant
-                                  SINVAR_LIB_SubnetsInGW
+                                  METASINVAR_SystemBoundary
                                     \<lparr> node_properties = C_host_attributes \<rparr>"
 end
 
@@ -119,7 +119,7 @@ ML_val{*
 visualize_edges @{context} @{term "edgesL policy"}
     [("edge [dir=\"arrow\", style=dashed, color=\"#FF8822\", constraint=false]",
      @{term "[(e1, e2) \<leftarrow>  List.product  (nodesL policy) (nodesL policy).
-     ((e1,e2) \<notin> set (edgesL policy)) \<and> ((e1,e2) \<notin> set( edgesL (make_policy invariants (nodesL policy)))) \<and> (e2 = V ''Adversary'') \<and> (e1 \<noteq> V ''Adversary'')]"})] "";
+     ((e1,e2) \<notin> set (edgesL policy)) \<and> ((e1,e2) \<notin> set( edgesL (make_policy invariants (nodesL policy)))) \<and> (e2 = ''Adversary'') \<and> (e1 \<noteq> ''Adversary'')]"})] "";
 *}
 
 
